CslibTests/ReductionSystem.lean
@@ -3,13 +3,18 @@ import Cslib.Semantics.ReductionSystem.Basic
 @[reduction_sys rs "ₙ", simp]
 def PredReduction (a b : ℕ) : Prop := a = b + 1
 
-open Relation.ReflTransGen
-
 lemma single_step : 5 ⭢ₙ 4 := by
   change PredReduction _ _
   simp
 
-lemma multiple_step : 5 ↠ₙ 3 := by
+-- `Trans` instances allow us to switch between single and multistep reductions in a `calc` block
+lemma multiple_step : 5 ↠ₙ 1 := by
+  -- TODO: can/should this be a `simp` attribute somewhere?
+  have h : rs.Red = PredReduction := by rfl
   calc
-    5 ↠ₙ 4 := by apply single; change PredReduction _ _; simp
-    _ ↠ₙ 3 := by apply single; change PredReduction _ _; simp
+    5 ⭢ₙ 4 := by simp [h]
+    _ ↠ₙ 2 := by
+      calc
+        4 ⭢ₙ 3 := by simp [h]
+        _ ⭢ₙ 2 := by simp [h]
+    _ ⭢ₙ 1 := by simp [h]
